SSL-Coq/less-than-one-a-press/proofs/InkFloorListEffects.v
@@ -1,0 +1,172 @@
+(** The real floor-list traversal only writes its height output. This covers
+    every completed generated US/JP traversal, including early rejection,
+    camera filters and list order. It does not identify the selected floor. *)
+From Coq Require Import Bool Lia List ZArith.
+From compcert Require Import AST Clight ClightBigstep Clightdefs Cop Ctypes
+  Events Globalenvs Integers Maps Memory Values.
+From LessThanOneAPress.Proofs Require Import GameTypes ObjectContactNecessity
+  ContactConsumerExecution UpperElevatorQueryResolution.
+Import ListNotations.
+Import Clightdefs.ClightNotations.
+Local Open Scope Z_scope.
+Module IFL := UEQR_UC.
+
+(** A structural induction over actual Clight executions. Both semantic
+    write/call obligations below are discharged for the floor helpers. *)
+Fixpoint ifl_shape keep (write_ok : expr -> bool)
+    (call_ok : expr -> list expr -> bool) (s : statement) : bool :=
+  match s with
+  | Sskip | Sbreak | Scontinue | Sreturn _ => true
+  | Sset id _ => negb (Pos.eqb id keep)
+  | Sassign lhs _ => write_ok lhs
+  | Scall opt fn args =>
+      (match opt with None => true | Some id => negb (Pos.eqb id keep) end)
+        && call_ok fn args
+  | Ssequence a b | Sifthenelse _ a b | Sloop a b =>
+      ifl_shape keep write_ok call_ok a && ifl_shape keep write_ok call_ok b
+  | _ => false
+  end.
+
+Lemma ifl_set_keep : forall (le : temp_env) id keep v,
+  negb (Pos.eqb id keep) = true -> (PTree.set id v le) ! keep = le ! keep.
+Proof.
+  intros. apply negb_true_iff in H. apply Pos.eqb_neq in H.
+  apply PTree.gso. congruence.
+Qed.
+
+Theorem ifl_checked_frame : forall ge e keep pointer (observe : mem -> option val)
+    write_ok call_ok,
+  (forall le m lhs rhs t le' m' out,
+    le ! keep = Some pointer -> write_ok lhs = true ->
+    ocn_exec ge e le m (Sassign lhs rhs) t le' m' out ->
+    t = E0 /\ observe m' = observe m) ->
+  (forall le m opt fn args t le' m' out,
+    le ! keep = Some pointer -> call_ok fn args = true ->
+    ocn_exec ge e le m (Scall opt fn args) t le' m' out ->
+    t = E0 /\ observe m' = observe m) ->
+  forall le m s t le' m' out,
+    ocn_exec ge e le m s t le' m' out ->
+    ifl_shape keep write_ok call_ok s = true -> le ! keep = Some pointer ->
+    t = E0 /\ observe m' = observe m /\ le' ! keep = Some pointer.
+Proof.
+  intros ge e keep pointer observe write_ok call_ok Hwrite Hcall
+    le m s t le' m' out Hrun.
+  induction Hrun; cbn [ifl_shape]; intros Hshape Hkeep; try discriminate;
+    try solve [repeat split; auto].
+  - destruct (Hwrite _ _ _ _ _ _ _ _ Hkeep Hshape ltac:(econstructor; eauto)).
+    auto.
+  - repeat split; auto. rewrite ifl_set_keep by exact Hshape. exact Hkeep.
+  - apply andb_true_iff in Hshape as [Hfresh Hallowed].
+    destruct (Hcall le m optid a al t (set_opttemp optid vres le) m' Out_normal
+      Hkeep Hallowed ltac:(econstructor; eauto)).
+    repeat split; auto. destruct optid; cbn; auto.
+    rewrite ifl_set_keep by exact Hfresh. exact Hkeep.
+  - apply andb_true_iff in Hshape as [Ha Hb].
+    destruct (IHHrun1 Hwrite Hcall Ha Hkeep) as (-> & Hfirst & Hmiddle).
+    destruct (IHHrun2 Hwrite Hcall Hb Hmiddle) as (-> & Hsecond & Hfinal).
+    repeat split; auto; congruence.
+  - apply andb_true_iff in Hshape as [Ha Hb]. auto.
+  - apply andb_true_iff in Hshape as [Ha Hb]. destruct b; auto.
+  - apply andb_true_iff in Hshape as [Ha Hb]. auto.
+  - apply andb_true_iff in Hshape as [Ha Hb].
+    destruct (IHHrun1 Hwrite Hcall Ha Hkeep) as (-> & Hfirst & Hmiddle).
+    destruct (IHHrun2 Hwrite Hcall Hb Hmiddle) as (-> & Hsecond & Hfinal).
+    repeat split; auto; congruence.
+  - apply andb_true_iff in Hshape as [Ha Hb].
+    destruct (IHHrun1 Hwrite Hcall Ha Hkeep) as (-> & Hfirst & Hmiddle).
+    destruct (IHHrun2 Hwrite Hcall Hb Hmiddle) as (-> & Hsecond & Hnext).
+    destruct (IHHrun3 Hwrite Hcall (andb_true_intro (conj Ha Hb)) Hnext)
+      as (-> & Hthird & Hfinal).
+    repeat split; auto; congruence.
+  Unshelve. all: exact None.
+Qed.
+
+Definition ifl_pointer_write id ty lhs := match lhs with
+  | Ederef (Etempvar found pty) actual =>
+      Pos.eqb found id &&
+      (if type_eq pty (tptr ty) then if type_eq actual ty then true else false else false)
+  | _ => false end.
+
+Lemma ifl_pointer_write_exact : forall id ty lhs,
+  ifl_pointer_write id ty lhs = true -> lhs = Ederef (Etempvar id (tptr ty)) ty.
+Proof.
+  intros id ty lhs. destruct lhs; try discriminate.
+  destruct lhs; try discriminate. cbn [ifl_pointer_write].
+  intro H. apply andb_true_iff in H as [Hid Htypes]. apply Pos.eqb_eq in Hid.
+  destruct (type_eq t0 (tptr ty)); try discriminate.
+  destruct (type_eq t ty); try discriminate. subst. reflexivity.
+Qed.
+
+Lemma ifl_pointer_store : forall ge e le m id ty chunk b ofs rhs t le' m' out,
+  le ! id = Some (Vptr b ofs) -> access_mode ty = By_value chunk ->
+  ocn_exec ge e le m (Sassign (Ederef (Etempvar id (tptr ty)) ty) rhs) t le' m' out ->
+  t = E0 /\ exists value, Mem.store chunk m b (Ptrofs.unsigned ofs) value = Some m'.
+Proof.
+  intros ge e le m id ty chunk b ofs rhs t le' m' out Hptr Hmode Hrun.
+  inversion Hrun; subst.
+  match goal with Hl : eval_lvalue _ _ _ _ (Ederef _ _) _ _ _ |- _ =>
+    inversion Hl; subst; clear Hl end.
+  match goal with Hr : eval_expr _ _ _ _ (Etempvar id _) ?value |- _ =>
+    assert (value = Vptr b ofs) as Hvalue by (eapply ocn_temp_value; eauto);
+    inversion Hvalue; subst end.
+  match goal with Ha : assign_loc _ _ _ _ _ _ _ _ |- _ =>
+    cbn [typeof] in Ha;
+    inversion Ha; subst; try congruence end.
+  match goal with Haccess : access_mode ty = By_value _ |- _ =>
+    rewrite Hmode in Haccess; inversion Haccess; subst end.
+  split; [reflexivity|]. eexists; eassumption.
+Qed.
+
+Definition ifl_disjoint (target : block) offset length chunk (b : block) ofs :=
+  b <> target \/ ofs + size_chunk chunk <= offset \/ offset + length <= ofs.
+
+Lemma ifl_source : forall version,
+  fn_vars (ueqr_native_body version UEQRFindFloorFromList) = [] /\
+  fn_params (ueqr_native_body version UEQRFindFloorFromList) =
+    [(IFL._surfaceNode, tptr (Tstruct IFL._SurfaceNode noattr));
+     (IFL._x, tint); (IFL._y, tint); (IFL._z, tint); (IFL._pheight, tptr tfloat)] /\
+  ifl_shape IFL._pheight (ifl_pointer_write IFL._pheight tfloat) (fun _ _ => false)
+    (fn_body (ueqr_native_body version UEQRFindFloorFromList)) = true.
+Proof. intros []; repeat split; reflexivity. Qed.
+
+Theorem ifl_completed_list_only_writes_height :
+  forall version ge m node x y z hb ho t m' result,
+  ClightBigstep.Clight2.eval_funcall ge m
+    (Internal (ueqr_native_body version UEQRFindFloorFromList))
+    [node; x; y; z; Vptr hb ho] t m' result ->
+  t = E0 /\ forall chunk b ofs,
+    ifl_disjoint hb (Ptrofs.unsigned ho) 4 chunk b ofs ->
+    Mem.load chunk m' b ofs = Mem.load chunk m b ofs.
+Proof.
+  intros version ge m node x y z hb ho t m' result Hcall.
+  destruct (ifl_source version) as (Hvars & Hparams & Hshape).
+  inversion Hcall; subst.
+  match goal with He : function_entry2 _ _ _ _ _ _ _ |- _ =>
+    inversion He; subst; clear He end.
+  match goal with Ha : alloc_variables _ _ _ _ _ _ |- _ =>
+    rewrite Hvars in Ha; inversion Ha; subst; clear Ha end.
+  match goal with Hfree : Mem.free_list ?before (blocks_of_env _ empty_env) = Some ?after |- _ =>
+    change (Some before = Some after) in Hfree; inversion Hfree; subst end.
+  match goal with Hb : bind_parameter_temps _ _ _ = Some ?temps |- _ =>
+    assert (temps ! IFL._pheight = Some (Vptr hb ho)) as Hptr by
+      (rewrite Hparams in Hb; cbn in Hb; inversion Hb; apply PTree.gss) end.
+  match goal with Hr : ClightBigstep.exec_stmt _ _ _ _ ?initial (fn_body _) _ _ _ _ |- _ =>
+    rename initial into m end.
+  assert (forall chunk b ofs, ifl_disjoint hb (Ptrofs.unsigned ho) 4 chunk b ofs ->
+    t = E0 /\ Mem.load chunk m' b ofs = Mem.load chunk m b ofs) as Hframe.
+  { intros chunk b ofs Hseparate.
+    lazymatch goal with Hr : ClightBigstep.exec_stmt _ _ _ _ _ (fn_body _) _ _ _ _ |- _ =>
+      destruct (ifl_checked_frame ge empty_env IFL._pheight (Vptr hb ho)
+        (fun memory => Mem.load chunk memory b ofs)
+        (ifl_pointer_write IFL._pheight tfloat) (fun _ _ => false)
+        ltac:(intros temps memory lhs rhs tr last after outcome Hp Hw Hs;
+          apply ifl_pointer_write_exact in Hw; subst lhs;
+          destruct (ifl_pointer_store _ _ _ _ _ tfloat Mfloat32 _ _ _ _ _ _ _ Hp eq_refl Hs)
+            as (Ht & value & Hstore); split; [exact Ht|];
+          eapply Mem.load_store_other; [exact Hstore|exact Hseparate])
+        ltac:(intros; discriminate) _ _ _ _ _ _ _ Hr Hshape Hptr)
+        as (Ht & Hloads & _); auto end. }
+  split.
+  - exact (proj1 (Hframe Mfloat32 hb (Ptrofs.unsigned ho + 4) ltac:(right; right; lia))).
+  - intros chunk b ofs Hdisjoint; exact (proj2 (Hframe _ _ _ Hdisjoint)).
+Qed.
